improve skeleton

ems/Skeleton.v
@@ -45,10 +45,10 @@ Qed.
 
 
 Module SkEnv.
+  Notation mblock := nat (only parsing).
+  Notation ptrofs := Z (only parsing).
 
-  Class t: Type := mk {
-    mblock: Type;
-    ptrofs: Type;
+  Record t: Type := mk {
     blk2id: mblock -> option gname;
     id2blk: gname -> option mblock;
   }
@@ -56,7 +56,6 @@ Module SkEnv.
 
   Definition wf (ske: t): Prop :=
     forall id blk, ske.(id2blk) id = Some blk <-> ske.(blk2id) blk = Some id.
-
 End SkEnv.
 
 
@@ -65,6 +64,7 @@ End SkEnv.
 
 
 Require Import Orders.
+Require Import Any.
 
 Module Sk.
   Class ld: Type := mk {
@@ -85,209 +85,205 @@ Module Sk.
     extends := fun a b => exists ctx, canon (add a ctx) = b;
   }
   .
+  
+  Module GDef <: Typ. Definition t := Any.t. End GDef.
+
+  Module SkSort := AListSort GDef.
+
+  Definition sort: alist gname Any.t -> alist gname Any.t := SkSort.sort.
+
+  Program Definition gdefs: ld :=
+    @mk (alist gname Any.t) nil (@List.app _) sort (fun sk => @List.NoDup _ (List.map fst sk)) _ _ _ _ _ _ _.
+  Next Obligation.
+  Proof.
+    eapply SkSort.sort_add_comm. auto.
+    (* eapply Permutation.Permutation_NoDup; [|et]. *)
+    (* eapply Permutation.Permutation_map. *)
+    (* symmetry. eapply SkSort.sort_permutation. *)
+  Qed.
+  Next Obligation.
+  Proof.
+    eapply List.app_assoc.
+  Qed.
+  Next Obligation.
+  Proof.
+    rewrite List.app_nil_r. auto.
+  Qed.
+  Next Obligation.
+  Proof.
+    i. eapply Permutation.Permutation_NoDup; [|et].
+    eapply Permutation.Permutation_map.
+    apply Permutation.Permutation_app_comm.
+  Qed.
+  Next Obligation.
+  Proof.
+    econs.
+  Qed.
+  Next Obligation.
+  Proof.
+    cut (NoDup (map fst a)).
+    { i. eapply Permutation.Permutation_NoDup; [|et].
+      eapply Permutation.Permutation_map.
+      eapply SkSort.sort_permutation. }
+    cut (NoDup (map fst (a ++ b))).
+    { i. rewrite map_app in H0.
+      eapply nodup_app_l. et. }
+    i. eapply Permutation.Permutation_NoDup; [|et].
+    eapply Permutation.Permutation_map.
+    symmetry. eapply SkSort.sort_permutation.
+  Qed.
+
+  Local Existing Instance gdefs.
+
+  Definition sort_add_comm sk0 sk1
+             (WF: wf (add sk0 sk1))
+    :
+      sort (add sk0 sk1) = sort (add sk1 sk0).
+  Proof.
+    eapply SkSort.sort_add_comm. eapply WF.
+  Qed.
+
+  Definition sort_wf sk (WF: wf sk):
+    wf (sort sk).
+  Proof.
+    ss. eapply Permutation.Permutation_NoDup; [|apply WF].
+    eapply Permutation.Permutation_map.
+    eapply SkSort.sort_permutation.
+  Qed.
+
+  (*** TODO: It might be nice if Sk.t also constitutes a resource algebra ***)
+  (*** At the moment, List.app is not assoc/commutative. We need to equip RA with custom equiv. ***)
+
+  Definition load_skenv (sk: t): (SkEnv.t) :=
+    let n := List.length sk in
+    {|
+      SkEnv.blk2id := fun blk => do '(gn, _) <- (List.nth_error sk blk); Some gn;
+      SkEnv.id2blk := fun id => do '(blk, _) <- find_idx (fun '(id', _) => string_dec id id') sk; Some blk
+    |}
+  .
+
+  Lemma load_skenv_wf
+        sk
+        (WF: wf sk)
+    :
+      <<WF: SkEnv.wf (load_skenv sk)>>
+  .
+  Proof.
+    r in WF.
+    rr. split; i; ss.
+    - uo; des_ifs.
+      + f_equal. ginduction sk; ss. i. inv WF.
+        rewrite find_idx_red in Heq1. des_ifs; ss.
+        { des_sumbool. subst. ss. clarify. }
+        des_sumbool. uo. des_ifs. destruct p. ss.
+        hexploit IHsk; et.
+      + exfalso. ginduction sk; ss. i. inv WF.
+        rewrite find_idx_red in Heq2. des_ifs; ss.
+        des_sumbool. uo. des_ifs. destruct p. ss.
+        hexploit IHsk; et.
+    - ginduction sk; ss.
+      { i. uo. ss. destruct blk; ss. }
+      i. destruct a. inv WF. uo. destruct blk; ss; clarify.
+      {  rewrite find_idx_red. uo. des_ifs; des_sumbool; ss. }
+      hexploit IHsk; et. i.
+      rewrite find_idx_red. uo. des_ifs; des_sumbool; ss. exfalso.
+      subst. clear - Heq1 H2. ginduction sk; ss. i.
+      rewrite find_idx_red in Heq1. des_ifs; des_sumbool; ss; et.
+      uo. des_ifs. destruct p. eapply IHsk; et.
+  Qed.
+
+  Definition incl (sk0 sk1: Sk.t): Prop :=
+    forall gn gd (IN: List.In (gn, gd) sk0),
+      List.In (gn, gd) sk1.
+
+  Program Instance incl_PreOrder: PreOrder incl.
+  Next Obligation.
+  Proof.
+    ii. ss.
+  Qed.
+  Next Obligation.
+  Proof.
+    ii. eapply H0. eapply H. ss.
+  Qed.
+
+  Lemma sort_incl sk
+    :
+      incl sk (sort sk).
+  Proof.
+    ii. eapply Permutation.Permutation_in; [|apply IN].
+    eapply SkSort.sort_permutation.
+  Qed.
+
+  Lemma sort_incl_rev sk
+    :
+      incl (sort sk) sk.
+  Proof.
+    ii. eapply Permutation.Permutation_in; [|apply IN].
+    symmetry. eapply SkSort.sort_permutation.
+  Qed.
+
+  Definition incl_env (sk0: Sk.t) (skenv: SkEnv.t): Prop :=
+    forall gn gd (IN: List.In (gn, gd) sk0),
+    exists blk, <<FIND: skenv.(SkEnv.id2blk) gn = Some blk>>.
+
+  Lemma incl_incl_env sk0 sk1
+        (INCL: incl sk0 sk1)
+    :
+      incl_env sk0 (load_skenv sk1).
+  Proof.
+    ii. exploit INCL; et. i. ss. uo. des_ifs; et.
+    exfalso. clear - x0 Heq0. ginduction sk1; et.
+    i. ss. rewrite find_idx_red in Heq0. des_ifs.
+    des_sumbool. uo.  des_ifs. des; clarify.
+    eapply IHsk1; et.
+  Qed.
+
+  Lemma in_env_in_sk :
+    forall sk blk symb
+      (FIND: SkEnv.blk2id (load_skenv sk) blk = Some symb),
+    exists def, In (symb, def) sk.
+  Proof.
+    i. unfold SkEnv.blk2id. ss.
+    uo. des_ifs. des; clarify.
+    eapply nth_error_In in Heq0. et.
+  Qed.
+
+  Lemma in_sk_in_env :
+    forall sk def symb
+           (IN: In (symb, def) sk),
+    exists blk, SkEnv.blk2id (Sk.load_skenv sk) blk = Some symb.
+  Proof.
+    i. unfold SkEnv.blk2id. ss.
+    uo. eapply In_nth_error in IN. des.
+    eexists. rewrite IN. et.
+  Qed.
+
+  Lemma env_range_some :
+    forall sk blk
+      (BLKRANGE : blk < Datatypes.length sk),
+      <<FOUND : exists symb, SkEnv.blk2id (Sk.load_skenv sk) blk = Some symb>>.
+  Proof.
+    i. depgen sk. induction blk; i; ss; clarify.
+    { destruct sk; ss; clarify.
+      { lia. }
+      uo. destruct p. exists s. ss. }
+    destruct sk; ss; clarify.
+    { lia. }
+    apply lt_S_n in BLKRANGE. eapply IHblk; eauto.
+  Qed.
+
+  Lemma env_found_range :
+    forall sk symb blk
+      (FOUND : SkEnv.id2blk (Sk.load_skenv sk) symb = Some blk),
+      <<BLKRANGE : blk < Datatypes.length sk>>.
+  Proof.
+    induction sk; i; ss; clarify.
+    uo; des_ifs. destruct p0. rewrite find_idx_red in Heq0. des_ifs.
+    { apply Nat.lt_0_succ. }
+    destruct blk.
+    { apply Nat.lt_0_succ. }
+    uo. des_ifs. destruct p. ss. clarify. apply lt_n_S. eapply IHsk; eauto.
+    instantiate (1:=symb). rewrite Heq0. ss.
+  Qed.
+
 End Sk.
-
-
-  (* (* Imp Instance *) *)
-  (* Inductive gdef: Type := Gfun | Gvar (gv: Z). *)
-
-  (* Module GDef <: Typ. Definition t := gdef. End GDef. *)
-  (* Module SkSort := AListSort GDef. *)
-
-  (* Definition sort: alist gname gdef -> alist gname gdef := SkSort.sort. *)
-
-  (* Program Definition gdefs: ld := *)
-  (*   @mk (alist gname gdef) nil (@List.app _) sort (fun sk => @List.NoDup _ (List.map fst sk)) _ _ _ _ _ _ _. *)
-  (* Next Obligation. *)
-  (* Proof. *)
-  (*   eapply SkSort.sort_add_comm. auto. *)
-  (*   (* eapply Permutation.Permutation_NoDup; [|et]. *) *)
-  (*   (* eapply Permutation.Permutation_map. *) *)
-  (*   (* symmetry. eapply SkSort.sort_permutation. *) *)
-  (* Qed. *)
-  (* Next Obligation. *)
-  (* Proof. *)
-  (*   eapply List.app_assoc. *)
-  (* Qed. *)
-  (* Next Obligation. *)
-  (* Proof. *)
-  (*   rewrite List.app_nil_r. auto. *)
-  (* Qed. *)
-  (* Next Obligation. *)
-  (* Proof. *)
-  (*   i. eapply Permutation.Permutation_NoDup; [|et]. *)
-  (*   eapply Permutation.Permutation_map. *)
-  (*   apply Permutation.Permutation_app_comm. *)
-  (* Qed. *)
-  (* Next Obligation. *)
-  (* Proof. *)
-  (*   econs. *)
-  (* Qed. *)
-  (* Next Obligation. *)
-  (* Proof. *)
-  (*   cut (NoDup (map fst a)). *)
-  (*   { i. eapply Permutation.Permutation_NoDup; [|et]. *)
-  (*     eapply Permutation.Permutation_map. *)
-  (*     eapply SkSort.sort_permutation. } *)
-  (*   cut (NoDup (map fst (a ++ b))). *)
-  (*   { i. rewrite map_app in H0. *)
-  (*     eapply nodup_app_l. et. } *)
-  (*   i. eapply Permutation.Permutation_NoDup; [|et]. *)
-  (*   eapply Permutation.Permutation_map. *)
-  (*   symmetry. eapply SkSort.sort_permutation. *)
-  (* Qed. *)
-
-  (* Local Existing Instance gdefs. *)
-
-  (* Definition sort_add_comm sk0 sk1 *)
-  (*            (WF: wf (add sk0 sk1)) *)
-  (*   : *)
-  (*     sort (add sk0 sk1) = sort (add sk1 sk0). *)
-  (* Proof. *)
-  (*   eapply SkSort.sort_add_comm. eapply WF. *)
-  (* Qed. *)
-
-
-  (* Definition sort_wf sk (WF: wf sk): *)
-  (*   wf (sort sk). *)
-  (* Proof. *)
-  (*   ss. eapply Permutation.Permutation_NoDup; [|apply WF]. *)
-  (*   eapply Permutation.Permutation_map. *)
-  (*   eapply SkSort.sort_permutation. *)
-  (* Qed. *)
-
-  (* (*** TODO: It might be nice if Sk.t also constitutes a resource algebra ***) *)
-  (* (*** At the moment, List.app is not assoc/commutative. We need to equip RA with custom equiv. ***) *)
-
-  (* Definition load_skenv (sk: t): (SkEnv.t) := *)
-  (*   let n := List.length sk in *)
-  (*   {| *)
-  (*     SkEnv.blk2id := fun blk => do '(gn, _) <- (List.nth_error sk blk); Some gn; *)
-  (*     SkEnv.id2blk := fun id => do '(blk, _) <- find_idx (fun '(id', _) => string_dec id id') sk; Some blk *)
-  (*   |} *)
-  (* . *)
-
-  (* Lemma load_skenv_wf *)
-  (*       sk *)
-  (*       (WF: wf sk) *)
-  (*   : *)
-  (*     <<WF: SkEnv.wf (load_skenv sk)>> *)
-  (* . *)
-  (* Proof. *)
-  (*   r in WF. *)
-  (*   rr. split; i; ss. *)
-  (*   - uo; des_ifs. *)
-  (*     + f_equal. ginduction sk; ss. i. inv WF. *)
-  (*       rewrite find_idx_red in Heq1. des_ifs; ss. *)
-  (*       { des_sumbool. subst. ss. clarify. } *)
-  (*       des_sumbool. uo. des_ifs. destruct p. ss. *)
-  (*       hexploit IHsk; et. *)
-  (*     + exfalso. ginduction sk; ss. i. inv WF. *)
-  (*       rewrite find_idx_red in Heq2. des_ifs; ss. *)
-  (*       des_sumbool. uo. des_ifs. destruct p. ss. *)
-  (*       hexploit IHsk; et. *)
-  (*   - ginduction sk; ss. *)
-  (*     { i. uo. ss. destruct blk; ss. } *)
-  (*     i. destruct a. inv WF. uo. destruct blk; ss; clarify. *)
-  (*     {  rewrite find_idx_red. uo. des_ifs; des_sumbool; ss. } *)
-  (*     hexploit IHsk; et. i. *)
-  (*     rewrite find_idx_red. uo. des_ifs; des_sumbool; ss. exfalso. *)
-  (*     subst. clear - Heq1 H2. ginduction sk; ss. i. *)
-  (*     rewrite find_idx_red in Heq1. des_ifs; des_sumbool; ss; et. *)
-  (*     uo. des_ifs. destruct p. eapply IHsk; et. *)
-  (* Qed. *)
-
-  (* Definition incl (sk0 sk1: Sk.t): Prop := *)
-  (*   forall gn gd (IN: List.In (gn, gd) sk0), *)
-  (*     List.In (gn, gd) sk1. *)
-
-  (* Program Instance incl_PreOrder: PreOrder incl. *)
-  (* Next Obligation. *)
-  (* Proof. *)
-  (*   ii. ss. *)
-  (* Qed. *)
-  (* Next Obligation. *)
-  (* Proof. *)
-  (*   ii. eapply H0. eapply H. ss. *)
-  (* Qed. *)
-
-  (* Lemma sort_incl sk *)
-  (*   : *)
-  (*     incl sk (sort sk). *)
-  (* Proof. *)
-  (*   ii. eapply Permutation.Permutation_in; [|apply IN]. *)
-  (*   eapply SkSort.sort_permutation. *)
-  (* Qed. *)
-
-  (* Lemma sort_incl_rev sk *)
-  (*   : *)
-  (*     incl (sort sk) sk. *)
-  (* Proof. *)
-  (*   ii. eapply Permutation.Permutation_in; [|apply IN]. *)
-  (*   symmetry. eapply SkSort.sort_permutation. *)
-  (* Qed. *)
-
-  (* Definition incl_env (sk0: Sk.t) (skenv: SkEnv.t): Prop := *)
-  (*   forall gn gd (IN: List.In (gn, gd) sk0), *)
-  (*   exists blk, <<FIND: skenv.(SkEnv.id2blk) gn = Some blk>>. *)
-
-  (* Lemma incl_incl_env sk0 sk1 *)
-  (*       (INCL: incl sk0 sk1) *)
-  (*   : *)
-  (*     incl_env sk0 (load_skenv sk1). *)
-  (* Proof. *)
-  (*   ii. exploit INCL; et. i. ss. uo. des_ifs; et. *)
-  (*   exfalso. clear - x0 Heq0. ginduction sk1; et. *)
-  (*   i. ss. rewrite find_idx_red in Heq0. des_ifs. *)
-  (*   des_sumbool. uo.  des_ifs. des; clarify. *)
-  (*   eapply IHsk1; et. *)
-  (* Qed. *)
-
-  (* Lemma in_env_in_sk : *)
-  (*   forall sk blk symb *)
-  (*     (FIND: SkEnv.blk2id (Sk.load_skenv sk) blk = Some symb), *)
-  (*   exists def, In (symb, def) sk. *)
-  (* Proof. *)
-  (*   i. unfold SkEnv.blk2id. ss. *)
-  (*   uo. des_ifs. des; clarify. *)
-  (*   eapply nth_error_In in Heq0. et. *)
-  (* Qed. *)
-
-  (* Lemma in_sk_in_env : *)
-  (*   forall sk def symb *)
-  (*          (IN: In (symb, def) sk), *)
-  (*   exists blk, SkEnv.blk2id (Sk.load_skenv sk) blk = Some symb. *)
-  (* Proof. *)
-  (*   i. unfold SkEnv.blk2id. ss. *)
-  (*   uo. eapply In_nth_error in IN. des. *)
-  (*   eexists. rewrite IN. et. *)
-  (* Qed. *)
-
-  (* Lemma env_range_some : *)
-  (*   forall sk blk *)
-  (*     (BLKRANGE : blk < Datatypes.length sk), *)
-  (*     <<FOUND : exists symb, SkEnv.blk2id (Sk.load_skenv sk) blk = Some symb>>. *)
-  (* Proof. *)
-  (*   i. depgen sk. induction blk; i; ss; clarify. *)
-  (*   { destruct sk; ss; clarify. *)
-  (*     { lia. } *)
-  (*     uo. destruct p. exists s. ss. } *)
-  (*   destruct sk; ss; clarify. *)
-  (*   { lia. } *)
-  (*   apply lt_S_n in BLKRANGE. eapply IHblk; eauto. *)
-  (* Qed. *)
-
-  (* Lemma env_found_range : *)
-  (*   forall sk symb blk *)
-  (*     (FOUND : SkEnv.id2blk (Sk.load_skenv sk) symb = Some blk), *)
-  (*     <<BLKRANGE : blk < Datatypes.length sk>>. *)
-  (* Proof. *)
-  (*   induction sk; i; ss; clarify. *)
-  (*   uo; des_ifs. destruct p0. rewrite find_idx_red in Heq0. des_ifs. *)
-  (*   { apply Nat.lt_0_succ. } *)
-  (*   destruct blk. *)
-  (*   { apply Nat.lt_0_succ. } *)
-  (*   uo. des_ifs. destruct p. ss. clarify. apply lt_n_S. eapply IHsk; eauto. *)
-  (*   instantiate (1:=symb). rewrite Heq0. ss. *)
-  (* Qed. *)
-
